examples WIP

theories/Dot/examples/examples.v
@@ -1,272 +1,39 @@
-From iris.proofmode Require Import tactics.
-From D.pure_program_logic Require Import lifting adequacy.
-From D.Dot Require Import unary_lr
-  lr_lemmas lr_lemmasNoBinding lr_lemmasDefs lr_lemmasPrim.
-From D.Dot Require Import skeleton fundamental.
-From D.Dot Require Import scalaLib hoas exampleInfra typingExInfra.
-
 Import hoasNotation.
-
-Example loopDefTyp Γ : Γ v⊢ₜ[ ∅ ] hclose (htv hloopDefV) : hclose hloopDefT.
-Proof.
-  apply (Subs_typed_nocoerce (hclose hloopDefTConcr)); mltcrush. cbv.
-
-  eapply App_typed; last var.
-  tcrush; varsub; lookup.
-Qed.
-
-Example loopFunTyp Γ : Γ v⊢ₜ[∅] hclose hloopFunTm : hclose ⊤ →: ⊥.
-Proof. have ? := loopDefTyp Γ; tcrush. Qed.
-
-Example loopTyp Γ : Γ v⊢ₜ[∅] hclose hloopTm : ⊥.
-Proof.
-  have ? := loopFunTyp Γ; apply (App_typed (T1 := ⊤)), (Subs_typed_nocoerce 𝐍); tcrush.
-Qed.
-
-(** XXX Not currently using olty. *)
 Module example.
 Section ex.
   Context `{HdlangG: dlangG Σ}.
-
-  Import stamp_transfer.
-
-  Lemma alloc {s sγ} φ : sγ !! s = None → allGs sγ ==∗ s ↝n[ 0 ] φ.
-  Proof.
-    iIntros (Hs) "Hsγ".
-    by iMod (leadsto_alloc φ Hs with "Hsγ") as (?) "[_ [_ $]]".
-  Qed.
-
-  Definition pos v := ∃ n, v = vnat n ∧ n > 0.
-  Definition ipos: hoEnvD Σ 0 := (λI args ρ v, ⌜ pos v ⌝).
-  Import ectxi_language ectx_language.
-
-(* Arguments dlang_ectx_lang : simpl never.
-Arguments dlang_ectxi_lang : simpl never. *)
-
-  Ltac wp_bin_base := iApply wp_bin; first eapply bin_op_syntype_sound; by [|constructor].
-  Ltac wp_bin := iApply wp_wand; [wp_bin_base | iIntros].
-  Tactic Notation "wp_bind" uconstr(p) := iApply (wp_bind (fill [p])).
-
-  Lemma wp_ge m n (Hge : m > n) : WP m > n {{ w, w ≡ true }}%I.
-  Proof. wp_bin. ev; simplify_eq/=. by case_decide. Qed.
-  Lemma wp_nge m n (Hnge : ¬ m > n) : WP m > n {{ w, w ≡ false }}%I.
-  Proof. wp_bin. ev; simplify_eq/=. by case_decide. Qed.
-
-  Lemma pos_wp ρ v : ipos vnil ρ v ⊢ WP v > 0 {{ w, w ≡ vbool true }}.
-  Proof. iDestruct 1 as %(n & -> & ?). by iApply wp_ge. Qed.
-
   Import swap_later_impl.
-  Context `{SwapPropI Σ}.
-  Lemma loopSemT: WP hclose hloopTm {{ _, False }}%I.
-  Proof.
-    iDestruct (fundamental_typed _ _ _ _ (loopTyp []) with "[]") as "H".
-    iApply wellMappedφ_empty.
-    iSpecialize ("H" $! ids with "[//]").
-    by rewrite hsubst_id /=.
-  Qed.
-
-  Definition hmkPosBodyV n := htif (n > 0) n hloopTm.
-  Definition hmkPosV := λ: n, hmkPosBodyV n.
-  Lemma wp_if_ge (n : nat) :
-    WP hclose (hmkPosBodyV n) {{ w, ⌜ w = n ∧ n > 0 ⌝}}%I.
-  Proof.
-    wp_bind (IfCtx _ _).
-    wp_bin; ev; simplify_eq/=.
-    case_decide; rewrite -wp_pure_step_later //; iNext.
-    by rewrite -wp_value'.
-    iApply wp_wand; [iApply loopSemT | naive_solver].
-  Qed.
-
-  Lemma wp_if_ge' (n : nat) :
-    WP tif (n > 0) (1 `div` n) (hclose hloopTm) {{ w, ⟦ 𝐍 ⟧ ids w ∧ ⌜ n > 0 ⌝}}%I.
-  Proof.
-    wp_bind (IfCtx _ _).
-    wp_bin; ev; simplify_eq/=.
-    case_decide; rewrite -wp_pure_step_later //; iNext.
-    - wp_bin. naive_solver.
-    - iApply wp_wand; [iApply loopSemT | naive_solver].
-  Qed.
-
-  Context (s: stamp).
-
-  Definition Hs := (s ↝n[ 0 ] ipos)%I.
-  Lemma allocHs sγ:
-    sγ !! s = None → allGs sγ ==∗ Hs.
-  Proof. exact (alloc ipos). Qed.
-
-  (* Experiments using fancier infrastructure: *)
-  Lemma allocHsGen sγ:
-    sγ !! s = None → allGs sγ ==∗ Hs.
-  Proof.
-    iIntros (Hl) "H". iApply wellMappedφ_apply;
-      last iApply (transfer (<[s:=ipos]> ∅) with "H") => s';
-      rewrite ?lookup_insert ?dom_insert ?dom_empty //; set_solver.
-  Qed.
-
-  Lemma allocHs1: allGs ∅ ==∗ Hs.
-  Proof.
-    iIntros "H"; iApply wellMappedφ_apply; last iApply (transfer_empty (<[s:=ipos]> ∅) with "H").
-    by rewrite lookup_insert.
-  Qed.
-
   (* Generic useful lemmas — not needed for fundamental theorem,
      but very useful for examples. *)
-  Lemma setp_value_eq (T : olty Σ 0) v: (∀ ρ, T vnil ρ v.[ρ]) ⊣⊢ [] s⊨ tv v : T.
-  Proof.
-    iSplit.
-    - iIntros "#H !>" (? _).
-      rewrite /= -wp_value'. iApply "H".
-    - iIntros "/= H" (ρ).
-      iSpecialize ("H" $! ρ with "[//]").
-      by rewrite /= wp_value_inv'.
-  Qed.
-
-  Lemma ietp_value_eq T v: (∀ ρ, ⟦ T ⟧ ρ v.[ρ]) ⊣⊢ [] ⊨ tv v : T.
-  Proof. apply setp_value_eq. Qed.
-
-  Lemma ietp_value T v: (∀ ρ, ⟦ T ⟧ ρ v.[ρ]) -∗ [] ⊨ tv v : T.
-  Proof. by rewrite ietp_value_eq. Qed.
-
-  Lemma ietp_value_inv T v: [] ⊨ tv v : T -∗ ∀ ρ, ⟦ T ⟧ ρ v.[ρ].
-  Proof. by rewrite ietp_value_eq. Qed.
 
   Import hoasNotation.
-
-  Definition posModT := μ: self, {@
-    type "Pos" >: ⊥ <: 𝐍;
-    val "mkPos" : 𝐍 →: self @; "Pos";
-    val "div" : 𝐍 →: self @; "Pos" →: 𝐍
-  }.
-
-  Definition hdivV := λ: m n, (htskip m) `div` n.
-
-  (** Under Iris assumption [Hs], [v.A] points to [ipos].
-      We assume [Hs] throughout the rest of the section. *)
+  (** Under Iris assumption [Hs], [v.A] points to [ipos]. *)
   Import DBNotation.
-
-  Definition posModV := ν {@
-    type "Pos" = ([]; s);
-    val "mkPos" = pv (hclose hmkPosV);
-    val "div" = pv (hclose hdivV)
-  }.
 
   Definition v := ν {@
     type "A" = ([]; s);
-	  val "n" = pv (vnat 2)
+    val "n" = pv (vnat 2)
   }.
-
-  Lemma sToIpos : Hs -∗ dtysem [] s ↗n[ 0 ] hoEnvD_inst [] ipos.
-  Proof. by iApply dm_to_type_intro. Qed.
-
-  Lemma sHasA : Hs -∗ oDTMem V⟦ ⊥ ⟧ V⟦ 𝐍 ⟧ ids (dtysem [] s).
-  Proof.
-    iIntros; cbn; repeat (repeat iExists _; repeat iSplit; try done).
-    by iApply sToIpos.
-    iModIntro; repeat iSplit; iIntros (w). by iIntros ">[]".
-    iMod 1 as %(n & -> & ?). iPureIntro.
-    rewrite /pure_interp_prim /prim_evals_to /=. eauto.
-  Qed.
-
-  (* Argh, no semantic "unTLater" yet. *)
-  Lemma sT_Forall_I {Γ} T1 T2 e:
-    shift T1 :: Γ s⊨ e : T2 -∗
-    (*─────────────────────────*)
-    Γ s⊨ tv (vabs e) : oAll T1 T2.
-  Proof.
-    iIntros "#HeT !>" (ρ) "#HG /= !>".
-    rewrite -wp_value'. iExists _; iSplit; first done.
-    iIntros "!>" (v) "#Hv"; rewrite up_sub_compose.
-    (* Factor ⪭ out of [G⟦ Γ ⟧ ρ] before [iNext]. *)
-    iNext.
-    iApply ("HeT" $! (v .: ρ) with "[$HG]").
-    by rewrite (hoEnvD_weaken_one (olty_car T1) _ _ _) stail_eq.
-  Qed.
-
-  Lemma ty_mkPos :
-    [] s⊨ hclose hmkPosV : oAll V⟦ 𝐍 ⟧ (olty0 (λI ρ v, ⌜ ∃ n : nat, v = n ∧ n > 0 ⌝)).
-  Proof.
-    rewrite -sT_Forall_I /= /shead.
-    iIntros (ρ) "!> /=". iDestruct 1 as %(_ & n & Hw); simplify_eq/=; rewrite Hw.
-    iIntros "!>". iApply wp_wand; [iApply wp_if_ge | naive_solver].
-  Qed.
-
-  Lemma wp_mkPos :
-    oAll V⟦ 𝐍 ⟧ (olty0 (λI ρ v, ⌜ ∃ n : nat, v = n ∧ n > 0 ⌝)) vnil ids (hclose hmkPosV).
-  Proof. iApply wp_value_inv'. iApply (ty_mkPos with "[//]"). Qed.
-
   (** Yes, v has a valid type member. *)
-  Lemma vHasA0: Hs -∗ ∀ ρ, ⟦ type "A" >: ⊥ <: TNat ⟧ ρ v.[ρ].
-  Proof.
-    iIntros "#Hs" (ρ); iExists _; iSplit; by [eauto | iApply sHasA].
-  Qed.
-
-  Lemma posModVHasAtyp: Hs -∗ [] ⊨ posModV : type "Pos" >: ⊥ <: TNat.
-  Proof.
-    rewrite -ietp_value; iIntros "#Hs" (ρ).
-    iExists _; iSplit; by [eauto | iApply sHasA].
-  Qed.
-
+  Arguments T_Sub {_ _ _ _ _ _ _}.
   Lemma vHasA0typ: Hs -∗ [] ⊨ tv v : type "A" >: ⊥ <: 𝐍.
-  Proof. rewrite -ietp_value. iApply vHasA0. Qed.
+  Proof.
+    iIntros "#Hs".
+    iApply (T_Sub (i := 0) (T1 := μ {@ type "A" >: ⊥ <: 𝐍})).
+    iApply T_New_I.
+    iApply DCons_I; [done| by iApply sHasA'|].
+    iSplit; [iIntros "!%"|iIntros "!> ** //"].
+    repeat constructor; exact: not_elem_of_nil.
+    iApply Sub_Trans.
+    iApply (Sub_Mu_A {@ type "A" >: ⊥ <: 𝐍}).
+    iApply And1_Sub.
+  Qed.
 
   Definition vTyp1Body : ty := {@
     type "A" >: ⊥ <: 𝐍;
     val "n" : p0 @; "A"
   }.
   Definition vTyp1 := μ vTyp1Body.
-
-  Lemma wp_div_spec (m : nat) w : ipos vnil ids w -∗ WP m `div` w {{ ⟦ 𝐍 ⟧ ids }}.
-  Proof. iDestruct 1 as %(n&?&?); simplify_eq. wp_bin. by iIntros "!%"; naive_solver. Qed.
-
-  Lemma V_TVMem_I T (v w : vl) l
-    (Hclv : nclosed_vl v 0)
-    (* XXX should be (Hlook : w @ l ↘ (dpt (pv v))) *)
-    (Hlook : objLookup v l (dpt (pv w))):
-    [] ⊨ tv w : T -∗
-    [] ⊨ v : TVMem l T.
-  Proof.
-    Import synLemmas.
-    have Hclw: nclosed_vl w 0.
-    by have := nclosed_lookup' Hlook Hclv; eauto with fv.
-    iIntros "#H"; iApply ietp_value; iIntros (ρ) "/=".
-    iSpecialize ("H" $! ρ with "[//]"). rewrite wp_value_inv.
-    rewrite !closed_subst_vl_id //.
-    do 2 (iExists _; iSplit; [done|]).
-    by rewrite path_wp_pv.
-  Qed.
-
-  Ltac valMember ρ :=
-    iApply V_TVMem_I; [solve_fv_congruence|naive_solver|
-      rewrite -ietp_value; iIntros (ρ)].
-
-  Lemma posModVHasA: Hs -∗ [] ⊨ posModV : hclose posModT.
-  Proof.
-    rewrite /posModT -(TMu_I _ posModV).
-    iIntros "#Hs". cbn -[ietp].
-    iApply TAnd_I; first by iApply posModVHasAtyp.
-    iApply TAnd_I; last iApply TAnd_I; last by
-      iIntros "!> ** /="; rewrite -wp_value'.
-    - valMember ρ; iExists _; iSplit; [done|].
-      iIntros (w) "!>"; iMod 1 as %[n Hw]; iIntros "!> !>".
-      simplify_eq/=.
-      iApply wp_wand; [iApply wp_if_ge | iIntros "/=" (v [-> ?])].
-      rewrite path_wp_pv.
-      repeat (iExists _; try iSplit => //=).
-      iSplit => //. by iApply dm_to_type_intro.
-      iIntros "!%"; rewrite /pos.
-      naive_solver.
-    - valMember ρ; iExists _; iSplit; [done|].
-      iIntros (v) "!>"; iMod 1 as %[m Hw]; iIntros "!> !>".
-      rewrite -wp_value'; simplify_eq/=; iExists _; iSplit; [done|].
-      iIntros (w) "!> #Harg!>!>"; rewrite path_wp_pv /=.
-      iDestruct "Harg" as (Φ d [ds Hlook]) "[Hs1 #Harg]";
-        have {d ds Hlook}->: d = dtysem [] s by naive_solver.
-      iPoseProof (sToIpos with "Hs") as "Hs2/=".
-      iPoseProof (dm_to_type_agree vnil w with "Hs1 Hs2") as "{Hs Hs1 Hs2} Heq".
-      wp_bind (BinLCtx _ _); rewrite -wp_pure_step_later // -wp_value/=/lang.of_val.
-      iNext. iRewrite "Heq" in "Harg"; iClear "Heq".
-      by iApply wp_div_spec.
-  Qed.
 
   (* This works. Crucially, we use TMu_I to introduce the object type.
      This way, we can inline the object in the type selection.
@@ -282,7 +49,7 @@ Arguments dlang_ectxi_lang : simpl never. *)
     iIntros "#Hs".
     iApply TAnd_I; first by [iApply vHasA0typ].
     iApply TAnd_I; first last.
-    - iApply (T_Sub _ _ _ _ 0); last by iApply Sub_Top.
+    - iApply (T_Sub (i := 0)); last by iApply Sub_Top.
       by iApply vHasA0typ.
     - rewrite -setp_value_eq /= /iPPred_car /=.
       have Hev2: pos (vnat 2) by rewrite /pos; eauto.
@@ -342,37 +109,11 @@ Arguments dlang_ectxi_lang : simpl never. *)
       "A" points to. *)
   Abort.
 
-  Lemma wp_prim_step {e : tm} (Hne : to_val e = None) φ :
-    WP e {{ φ }} ⊢ ∃ e2, ⌜ prim_step e tt [] e2 tt [] ⌝ ∧ ▷ WP e2 {{ φ }}.
+  (* Lemma vHasA1': Hs -∗ ∀ ρ, ⟦ vTyp1 ⟧ ρ v.[ρ].
   Proof.
-    rewrite wp_unfold/wp_pre/= {}Hne; iIntros "Hwp".
-    iDestruct ("Hwp" $! () [] [] 0 with "[//]") as (Hred) "Hwp".
-    destruct Hred as (? & e2 & [] & ? & Hr%prim_step_view).
-    iDestruct ("Hwp" $! e2 with "[%//]") as "(_ & Heq & _)".
-    by iExists _; iFrame.
-  Qed.
-
-  Lemma wp_head_step {e : tm} (Hsub : sub_redexes_are_values e) (Hne : to_val e = None) φ :
-    WP e {{ φ }} ⊢ ∃ e2 : tm, ⌜ head_step e tt [] e2 tt [] ⌝ ∧ ▷ WP e2 {{ φ }}.
-  Proof.
-    iIntros "H"; iDestruct (wp_prim_step Hne with "H") as (e2 Hred) "Hwp".
-    suff ?: head_step e () [] e2 () [] by iExists _; iFrame.
-    destruct Hred as [K]; subst; suff: K = [] by naive_solver.
-    by eapply Hsub, val_head_stuck.
-  Qed.
-
-  Lemma wp_pos ρ (v : vl) : WP v > 0 {{ w, w ≡ vbool true }} ⊢ ▷ ipos vnil ρ v.
-  Proof.
-    have Hsub: sub_redexes_are_values (v > 0). {
-      apply ectxi_language_sub_redexes_are_values.
-      by case => /= *; simplify_eq/=; eauto.
-    }
-    rewrite /ipos/pos (wp_head_step Hsub) //; iDestruct 1 as (e2 Hhr) "Heq"; iNext.
-    have {Hhr}[w [-> Hev]]: ∃ w : vl, e2 = w ∧ bin_op_eval blt 0 v = Some w by inverse Hhr; eauto.
-    iDestruct (wp_value_inv' with "Heq") as %->%leibniz_equiv; iIntros "!%".
-    (* rewrite wp_value_inv'; iDestruct "Heq" as %->%leibniz_equiv; iIntros "!%". *)
-    simpl in Hev; repeat case_match; repeat case_decide; naive_solver.
-  Qed.
+    rewrite -ietp_value_inv. iIntros "#Hs".
+    (* Fails, because we need a *syntactic* type. *)
+    iApply (T_Sub [] v _ vTyp1 0). *)
 
 End ex.
 
