theories/Dot/examples/semDiv.v
@@ -1,0 +1,442 @@
+From iris.proofmode Require Import tactics.
+From D.pure_program_logic Require Import lifting adequacy.
+From D.Dot Require Import unary_lr
+  lr_lemmas lr_lemmasNoBinding lr_lemmasDefs lr_lemmasPrim.
+From D.Dot Require Import typeExtractionSem.
+From D.Dot Require Import skeleton fundamental.
+From D.Dot Require Import scalaLib hoas exampleInfra typingExInfra.
+
+Import hoasNotation.
+
+Example loopDefTyp Γ : Γ v⊢ₜ[ ∅ ] hclose (htv hloopDefV) : hclose hloopDefT.
+Proof.
+  apply (Subs_typed_nocoerce (hclose hloopDefTConcr)); mltcrush. cbv.
+
+  eapply App_typed; last var.
+  tcrush; varsub; lookup.
+Qed.
+
+Example loopFunTyp Γ : Γ v⊢ₜ[∅] hclose hloopFunTm : hclose ⊤ →: ⊥.
+Proof. have ? := loopDefTyp Γ; tcrush. Qed.
+
+Example loopTyp Γ : Γ v⊢ₜ[∅] hclose hloopTm : ⊥.
+Proof.
+  have ? := loopFunTyp Γ; apply (App_typed (T1 := ⊤)), (Subs_typed_nocoerce 𝐍); tcrush.
+Qed.
+
+(** XXX Not currently using olty. *)
+Module examples.
+
+Import ectxi_language.
+
+Tactic Notation "wp_bind" uconstr(p) := iApply (wp_bind (fill [p])).
+Ltac wp_bin_base := iApply wp_bin; first eapply bin_op_syntype_sound; by [|constructor].
+Ltac wp_bin := iApply wp_wand; [wp_bin_base | iIntros].
+Tactic Notation "wp_bind" uconstr(p) := iApply (wp_bind (ectxi_language.fill [p])).
+Import stamp_transfer.
+
+(* Generic useful lemmas — not needed for fundamental theorem,
+    but very useful for examples. *)
+Section helpers.
+  Context `{HdlangG: dlangG Σ}.
+
+  Lemma alloc {s sγ} φ : sγ !! s = None → allGs sγ ==∗ s ↝n[ 0 ] φ.
+  Proof.
+    iIntros (Hs) "Hsγ".
+    by iMod (leadsto_alloc φ Hs with "Hsγ") as (?) "[_ [_ $]]".
+  Qed.
+  Lemma wp_ge m n (Hge : m > n) : WP m > n {{ w, w ≡ true }}%I.
+  Proof. wp_bin. ev; simplify_eq/=. by case_decide. Qed.
+  Lemma wp_nge m n (Hnge : ¬ m > n) : WP m > n {{ w, w ≡ false }}%I.
+  Proof. wp_bin. ev; simplify_eq/=. by case_decide. Qed.
+
+  (* Argh, no semantic "unTLater" yet. *)
+  Lemma sT_Forall_I {Γ} T1 T2 e:
+    shift T1 :: Γ s⊨ e : T2 -∗
+    (*─────────────────────────*)
+    Γ s⊨ tv (vabs e) : oAll T1 T2.
+  Proof.
+    iIntros "#HeT !>" (ρ) "#HG /= !>".
+    rewrite -wp_value'. iExists _; iSplit; first done.
+    iIntros "!>" (v) "#Hv"; rewrite up_sub_compose.
+    (* Factor ⪭ out of [G⟦ Γ ⟧ ρ] before [iNext]. *)
+    iNext.
+    iApply ("HeT" $! (v .: ρ) with "[$HG]").
+    by rewrite (hoEnvD_weaken_one (olty_car T1) _ _ _) stail_eq.
+  Qed.
+
+  Lemma setp_value_eq (T : olty Σ 0) v: (∀ ρ, T vnil ρ v.[ρ]) ⊣⊢ [] s⊨ tv v : T.
+  Proof.
+    iSplit.
+    - iIntros "#H !>" (? _).
+      rewrite /= -wp_value'. iApply "H".
+    - iIntros "/= H" (ρ).
+      iSpecialize ("H" $! ρ with "[//]").
+      by rewrite /= wp_value_inv'.
+  Qed.
+
+  Lemma ietp_value_eq T v: (∀ ρ, ⟦ T ⟧ ρ v.[ρ]) ⊣⊢ [] ⊨ tv v : T.
+  Proof. apply setp_value_eq. Qed.
+
+  Lemma ietp_value T v: (∀ ρ, ⟦ T ⟧ ρ v.[ρ]) -∗ [] ⊨ tv v : T.
+  Proof. by rewrite ietp_value_eq. Qed.
+
+  Lemma ietp_value_inv T v: [] ⊨ tv v : T -∗ ∀ ρ, ⟦ T ⟧ ρ v.[ρ].
+  Proof. by rewrite ietp_value_eq. Qed.
+End helpers.
+
+Section s_is_pos.
+
+Context `{HdlangG: dlangG Σ}.
+Context (s: stamp).
+
+Definition pos v := ∃ n, v = vnat n ∧ n > 0.
+Definition ipos: oltyO Σ 0 := olty0 (λI ρ v, ⌜ pos v ⌝).
+
+Definition Hs := (s ↝n[ 0 ] ipos)%I.
+Lemma allocHs sγ:
+  sγ !! s = None → allGs sγ ==∗ Hs.
+Proof. exact (alloc ipos). Qed.
+
+Section div_example.
+  Lemma idtp_value_eq T l d (Hl : label_of_ty T = Some l):
+    (∀ ρ, ⌜path_includes (pv (ids 0)) ρ [(l, d)]⌝ → D*⟦ T ⟧ ρ d.|[ρ]) ⊣⊢ [] s⊨ { l := d } : LD⟦ T ⟧.
+  Proof.
+    rewrite /idtp/=/lift_ldlty/=; iSplit.
+    by iIntros "#H !>" (ρ Hpid _); iFrame (Hl); iApply "H".
+    by iIntros "#H" (ρ Hpid); iDestruct ("H" $! ρ Hpid with "[//]") as "[_ $]".
+  Qed.
+
+  (* Arguments dlang_ectx_lang : simpl never.
+  Arguments dlang_ectxi_lang : simpl never. *)
+
+  Lemma pos_wp ρ v : ipos vnil ρ v ⊢ WP v > 0 {{ w, w ≡ vbool true }}.
+  Proof. iDestruct 1 as %(n & -> & ?). by iApply wp_ge. Qed.
+
+  Import swap_later_impl.
+  Context `{SwapPropI Σ}.
+  Lemma loopSemT: WP hclose hloopTm {{ _, False }}%I.
+  Proof.
+    iDestruct (fundamental_typed _ _ _ _ (loopTyp []) with "[]") as "H".
+    iApply wellMappedφ_empty.
+    iSpecialize ("H" $! ids with "[//]").
+    by rewrite hsubst_id /=.
+  Qed.
+
+  Definition hmkPosBodyV n := htif (n > 0) n hloopTm.
+  Definition hmkPosV := λ: n, hmkPosBodyV n.
+
+  Lemma wp_if_ge (n : nat) :
+    WP hclose (hmkPosBodyV n) {{ w, ⌜ w = n ∧ n > 0 ⌝}}%I.
+  Proof.
+    wp_bind (IfCtx _ _).
+    wp_bin; ev; simplify_eq/=.
+    case_decide; rewrite -wp_pure_step_later //; iNext.
+    by rewrite -wp_value'.
+    iApply wp_wand; [iApply loopSemT | naive_solver].
+  Qed.
+
+  Lemma wp_if_ge' (n : nat) :
+    WP tif (n > 0) (1 `div` n) (hclose hloopTm) {{ w, ⟦ 𝐍 ⟧ ids w ∧ ⌜ n > 0 ⌝}}%I.
+  Proof.
+    wp_bind (IfCtx _ _).
+    wp_bin; ev; simplify_eq/=.
+    case_decide; rewrite -wp_pure_step_later //; iNext.
+    - wp_bin. naive_solver.
+    - iApply wp_wand; [iApply loopSemT | naive_solver].
+  Qed.
+
+  (* Experiments using fancier infrastructure: *)
+  Lemma allocHsGen sγ:
+    sγ !! s = None → allGs sγ ==∗ Hs.
+  Proof.
+    (* iIntros (Hl) "H". iApply wellMappedφ_apply.
+    Fail pose (t := transfer (<[s:=ipos]> ∅)).
+    pose (u := transfer (<[s:=olty_car ipos]> ∅)).
+    2: iApply (transfer (<[s:=ipos]> ∅) with "H") => s'.
+      Unshelve. 3: apply _.
+    (* Check transfer (<[s:=olty_car ipos]> ∅). *)
+    Fail pose (t := transfer (<[s:=ipos]> ∅)). *)
+
+    iIntros (Hl) "H". iApply wellMappedφ_apply;
+      last iApply (transfer (<[s:=olty_car ipos]> ∅) with "H") => s';
+      rewrite ?lookup_insert ?dom_insert ?dom_empty //; set_solver.
+  Qed.
+
+  Lemma allocHs1: allGs ∅ ==∗ Hs.
+  Proof.
+    iIntros "H"; iApply wellMappedφ_apply; last iApply (transfer_empty (<[s:=olty_car ipos]> ∅) with "H").
+    by rewrite lookup_insert.
+  Qed.
+
+  Import hoasNotation.
+
+  Definition posModT := μ: self, {@
+    type "Pos" >: ⊥ <: 𝐍;
+    val "mkPos" : 𝐍 →: self @; "Pos";
+    val "div" : 𝐍 →: self @; "Pos" →: 𝐍
+  }.
+
+  Definition hdivV := λ: m n, (htskip m) `div` n.
+
+  (** We assume [Hs] throughout the rest of the section. *)
+  Import DBNotation.
+
+  Definition posModV := ν {@
+    type "Pos" = ([]; s);
+    val "mkPos" = pv (hclose hmkPosV);
+    val "div" = pv (hclose hdivV)
+  }.
+
+  Lemma sToIpos : Hs -∗ dtysem [] s ↗n[ 0 ] hoEnvD_inst [] ipos.
+  Proof. by iApply dm_to_type_intro. Qed.
+
+  Lemma sHasA' l Γ : Hs -∗ Γ s⊨ { l := dtysem [] s } : LD⟦ type l >: ⊥ <: 𝐍 ⟧.
+  Proof.
+    iIntros "Hs".
+    iApply (sD_Typ_Abs ipos); [|iApply Bot_Sub|by iExists _; iFrame "Hs"].
+    rewrite /ipos /pos/=; iIntros "!>" (ρ w) "_ >% !> !%".
+    rewrite /pure_interp_prim /prim_evals_to /=. naive_solver.
+  Qed.
+
+  Lemma sHasA l : Hs -∗ D*⟦ type l >: ⊥ <: 𝐍 ⟧ ids (dtysem [] s).
+  Proof.
+    iIntros; cbn; repeat (repeat iExists _; repeat iSplit; try done).
+    by iApply sToIpos.
+    iModIntro; repeat iSplit; iIntros (w). by iIntros ">[]".
+    iMod 1 as %(n & -> & ?). iPureIntro.
+    rewrite /pure_interp_prim /prim_evals_to /=. eauto.
+  Qed.
+
+  Lemma posModVHasAtyp: Hs -∗ [] ⊨ posModV : type "Pos" >: ⊥ <: TNat.
+  Proof.
+    rewrite -ietp_value; iIntros "#Hs" (ρ).
+    iExists _; iSplit; by [eauto | iApply (sHasA "Pos")].
+  Qed.
+
+
+  Lemma ty_mkPos :
+    [] s⊨ hclose hmkPosV : oAll V⟦ 𝐍 ⟧ (olty0 (λI ρ v, ⌜ ∃ n : nat, v = n ∧ n > 0 ⌝)).
+  Proof.
+    rewrite -sT_Forall_I /= /shead.
+    iIntros (ρ) "!> /=". iDestruct 1 as %(_ & n & Hw); simplify_eq/=; rewrite Hw.
+    iIntros "!>". iApply wp_wand; [iApply wp_if_ge | naive_solver].
+  Qed.
+
+  Lemma wp_mkPos :
+    oAll V⟦ 𝐍 ⟧ (olty0 (λI ρ v, ⌜ ∃ n : nat, v = n ∧ n > 0 ⌝)) vnil ids (hclose hmkPosV).
+  Proof. iApply wp_value_inv'. iApply (ty_mkPos with "[//]"). Qed.
+
+  Lemma wp_div_spec (m : nat) w : ipos vnil ids w -∗ WP m `div` w {{ ⟦ 𝐍 ⟧ ids }}.
+  Proof. iDestruct 1 as %(n&?&?); simplify_eq. wp_bin. by iIntros "!%"; naive_solver. Qed.
+
+  Lemma V_TVMem_I T (v w : vl) l
+    (Hclv : nclosed_vl v 0)
+    (* XXX should be (Hlook : w @ l ↘ (dpt (pv v))) *)
+    (Hlook : objLookup v l (dpt (pv w))):
+    [] ⊨ tv w : T -∗
+    [] ⊨ v : TVMem l T.
+  Proof.
+    Import synLemmas.
+    have Hclw: nclosed_vl w 0.
+    by have := nclosed_lookup' Hlook Hclv; eauto with fv.
+    iIntros "#H"; iApply ietp_value; iIntros (ρ) "/=".
+    iSpecialize ("H" $! ρ with "[//]"). rewrite wp_value_inv.
+    rewrite !closed_subst_vl_id //.
+    do 2 (iExists _; iSplit; [done|]).
+    by rewrite path_wp_pv.
+  Qed.
+
+  Ltac valMember ρ :=
+    iApply V_TVMem_I; [solve_fv_congruence|naive_solver|
+      rewrite -ietp_value; iIntros (ρ)].
+
+  Lemma posModVHasA: Hs -∗ [] ⊨ posModV : hclose posModT.
+  Proof.
+    rewrite /posModT -(TMu_I _ posModV).
+    iIntros "#Hs". cbn -[ietp].
+    iApply TAnd_I; first by iApply posModVHasAtyp.
+    iApply TAnd_I; last iApply TAnd_I; last by
+      iIntros "!> ** /="; rewrite -wp_value'.
+    - valMember ρ; iExists _; iSplit; [done|].
+      iIntros (w) "!>"; iMod 1 as %[n Hw]; iIntros "!> !>".
+      simplify_eq/=.
+      iApply wp_wand; [iApply wp_if_ge | iIntros "/=" (v [-> ?])].
+      rewrite path_wp_pv.
+      repeat (iExists _; try iSplit => //=).
+      iSplit => //. by iApply dm_to_type_intro.
+      iIntros "!%"; rewrite /pos.
+      naive_solver.
+    - valMember ρ; iExists _; iSplit; [done|].
+      iIntros (v) "!>"; iMod 1 as %[m Hw]; iIntros "!> !>".
+      rewrite -wp_value'; simplify_eq/=; iExists _; iSplit; [done|].
+      iIntros (w) "!> #Harg!>!>"; rewrite path_wp_pv /=.
+      iDestruct "Harg" as (Φ d [ds Hlook]) "[Hs1 #Harg]";
+        have {d ds Hlook}->: d = dtysem [] s by naive_solver.
+      iPoseProof (sToIpos with "Hs") as "Hs2/=".
+      iPoseProof (dm_to_type_agree vnil w with "Hs1 Hs2") as "{Hs Hs1 Hs2} Heq".
+      wp_bind (BinLCtx _ _); rewrite -wp_pure_step_later // -wp_value/=/lang.of_val.
+      iNext. iRewrite "Heq" in "Harg"; iClear "Heq".
+      by iApply wp_div_spec.
+  Qed.
+End div_example.
+
+Section wp_inv.
+  Import ectxi_language ectx_language.
+
+  Lemma wp_prim_step {e : tm} (Hne : to_val e = None) φ :
+    WP e {{ φ }} ⊢ ∃ e2, ⌜ prim_step e tt [] e2 tt [] ⌝ ∧ ▷ WP e2 {{ φ }}.
+  Proof.
+    rewrite wp_unfold/wp_pre/= {}Hne; iIntros "Hwp".
+    iDestruct ("Hwp" $! () [] [] 0 with "[//]") as (Hred) "Hwp".
+    destruct Hred as (? & e2 & [] & ? & Hr%prim_step_view).
+    iDestruct ("Hwp" $! e2 with "[%//]") as "(_ & Heq & _)".
+    by iExists _; iFrame.
+  Qed.
+
+  Lemma wp_head_step {e : tm} (Hsub : sub_redexes_are_values e) (Hne : to_val e = None) φ :
+    WP e {{ φ }} ⊢ ∃ e2 : tm, ⌜ head_step e tt [] e2 tt [] ⌝ ∧ ▷ WP e2 {{ φ }}.
+  Proof.
+    iIntros "H"; iDestruct (wp_prim_step Hne with "H") as (e2 Hred) "Hwp".
+    suff ?: head_step e () [] e2 () [] by iExists _; iFrame.
+    destruct Hred as [K]; subst; suff: K = [] by naive_solver.
+    by eapply Hsub, val_head_stuck.
+  Qed.
+
+  Lemma wp_pos ρ (v : vl) : WP v > 0 {{ w, w ≡ vbool true }} ⊢ ▷ ipos vnil ρ v.
+  Proof.
+    have Hsub: sub_redexes_are_values (v > 0). {
+      apply ectxi_language_sub_redexes_are_values.
+      by case => /= *; simplify_eq/=; eauto.
+    }
+    rewrite /ipos/pos (wp_head_step Hsub) //; iDestruct 1 as (e2 Hhr) "Heq"; iNext.
+    have {Hhr}[w [-> Hev]]: ∃ w : vl, e2 = w ∧ bin_op_eval blt 0 v = Some w by inverse Hhr; eauto.
+    iDestruct (wp_value_inv' with "Heq") as %->%leibniz_equiv; iIntros "!%".
+    (* rewrite wp_value_inv'; iDestruct "Heq" as %->%leibniz_equiv; iIntros "!%". *)
+    simpl in Hev; repeat case_match; repeat case_decide; naive_solver.
+  Qed.
+
+end wp_inv.
+
+Section small_ex.
+  (* Generic useful lemmas — not needed for fundamental theorem,
+     but very useful for examples. *)
+
+  (** Under Iris assumption [Hs], [v.A] points to [ipos]. *)
+  Import DBNotation.
+
+  Definition v := ν {@
+    type "A" = ([]; s);
+    val "n" = pv (vnat 2)
+  }.
+
+  Definition vTyp1Body : ty := {@
+    type "A" >: ⊥ <: 𝐍;
+    val "n" : p0 @; "A"
+  }.
+  Definition vTyp1 := μ vTyp1Body.
+
+
+  (** Yes, v has a valid type member. *)
+  Arguments T_Sub {_ _ _ _ _ _ _}.
+  Lemma vHasA0typ: Hs -∗ [] ⊨ tv v : type "A" >: ⊥ <: 𝐍.
+  Proof.
+    iIntros "#Hs".
+    iApply (T_Sub (i := 0) (T1 := μ {@ type "A" >: ⊥ <: 𝐍})).
+    iApply T_New_I.
+    iApply DCons_I; [done| by iApply sHasA'|].
+    iSplit; [iIntros "!%"|iIntros "!> ** //"].
+    repeat constructor; exact: not_elem_of_nil.
+    iApply Sub_Trans.
+    iApply (Sub_Mu_A {@ type "A" >: ⊥ <: 𝐍}).
+    iApply And1_Sub.
+  Qed.
+  (* This works. Crucially, we use TMu_I to introduce the object type.
+     This way, we can inline the object in the type selection.
+     This cannot be done using T_New_I directly.
+     However, this is closer to how typechecking in Scala
+     actually works.
+     XXX: also, maybe this *could* be done with T_New_I with
+     a precise type? That'd be a more correct derivation.
+   *)
+  Lemma vHasA1: Hs -∗ ∀ ρ, ⟦ vTyp1 ⟧ ρ v.[ρ].
+  Proof.
+    rewrite -ietp_value_inv -(TMu_I _ v).
+    iIntros "#Hs".
+    iApply TAnd_I; first by [iApply vHasA0typ].
+    iApply TAnd_I; first last.
+    - iApply (T_Sub (i := 0)); last by iApply Sub_Top.
+      by iApply vHasA0typ.
+    - rewrite -setp_value_eq /= /iPPred_car /=.
+      have Hev2: pos (vnat 2) by rewrite /pos; eauto.
+      iIntros (_).
+
+      repeat (repeat iExists _; repeat iSplit; rewrite ?path_wp_pv //);
+        try by [|iApply dm_to_type_intro].
+  Qed.
+
+  Lemma vHasA1t : Hs -∗ [] ⊨ tv v : vTyp1.
+  Proof. rewrite -ietp_value.
+  iApply vHasA1. Qed.
+
+  Lemma vHasA1TypAd : allGs ∅ ==∗ [] ⊨ tv v : vTyp1.
+  Proof. rewrite -ietp_value allocHs //; iIntros. by iApply vHasA1. Qed.
+
+  (* Lemma vHasA1': Hs -∗ ∀ ρ, ⟦ vTyp1 ⟧ ρ v.[ρ].
+  Proof.
+    rewrite -ietp_value_inv. iIntros "#Hs".
+    (* Fails, because we need a *syntactic* type. *)
+    iApply (T_Sub [] v _ vTyp1 0). *)
+
+  (*
+    A different approach would be to type the object using T_New_I
+    with an object type [U] with member [TTMem "A" ipos ipos].
+    We could then upcast the object. But type U is not syntactic,
+    so we can't express this yet using the existing typing
+    lemmas.
+    And if we use T_New_I on the final type, then [this.A]
+    is overly abstract when we try proving that [this.n : this.A];
+    see concretely below.
+  *)
+  Lemma vHasA1': Hs -∗ ⟦ vTyp1 ⟧ ids v.
+  Proof.
+    iIntros "#Hs".
+    iDestruct (T_New_I [] vTyp1Body with "[]") as "#H"; first last.
+    iSpecialize ("H" $! ids with "[#//]").
+    rewrite hsubst_id /interp_expr wp_value_inv'.
+    iApply "H".
+    iApply DCons_I => //.
+    - (* Can't finish with D_Typ_Abs, this is only for syntactic types: *)
+      (* From D.Dot Require Import typeExtractionSem.
+      iApply D_Typ_Abs => //; first last.
+      iExists _; iSplit => //=.  (* Here we need a syntactic type matching [ipos]. *) *)
+      iModIntro.
+      iIntros (ρ Hpid) "/= #_".
+      iSplit => //. by iApply sHasA.
+    - iApply DCons_I => //; last by iApply DNil_I.
+      iApply D_Path_TVMem_I.
+      iIntros "!>" (ρ) "/="; iDestruct 1 as "[_ [HA [HB _]]]".
+      iDestruct "HA" as (dA) "[HlA HA]".
+      iDestruct "HA" as (φ) "[Hlφ HA]".
+      iDestruct "HB" as (dB) "[HlB HB]".
+      iDestruct "HB" as (w) "HB".
+      rewrite !path_wp_pv.
+      iExists φ, dA; repeat iSplit => //; try iNext => //.
+      (* Last case is stuck, since we don't know what [ρ 0] is and what
+      "A" points to. *)
+  Abort.
+
+  (* Lemma vHasA1': Hs -∗ ∀ ρ, ⟦ vTyp1 ⟧ ρ v.[ρ].
+  Proof.
+    rewrite -ietp_value_inv. iIntros "#Hs".
+    (* Fails, because we need a *syntactic* type. *)
+    iApply (T_Sub [] v _ vTyp1 0). *)
+
+End small_ex.
+End s_is_pos.
+
+Import dlang_adequacy swap_later_impl.
+Lemma vSafe: safe (tv (v 1%positive)).
+Proof. eapply (safety_dot_sem dlangΣ)=>*; apply vHasA1TypAd. Qed.
+
+End examples.
